PDDL-sema/AST1.thy
@@ -3,161 +3,8 @@ theory AST1
   "HOL.Rat" 
   Util
 begin
-  
-type_synonym name = String.literal
 
-type_synonym pred = name
-type_synonym func = name
-type_synonym pref = name
-
-datatype type = Either (primitives: "name list") | Number
-
-datatype variable = Variable (var_name: name)
-
-datatype object = name: Object (obj_name: name)
-
-datatype var_num = Var variable | Num rat 
-datatype var_num_dur = Var variable | Num rat | Duration
-
-datatype symbol = Var variable | Const object | Num rat | Duration
-
-datatype instant_symbol = Var variable | Const object | Num rat
-
-datatype entity = Const object | Num rat
-
-find_theorems name: "Sum*type"
-
-datatype (sym: 'sym) "term" = 
-  Sym 'sym
-| Fun func (arguments: "'sym term list") 
-
-datatype (ent: 'ent) atom = 
-  Pred (pred: pred) (arguments: "'ent list")
-| Ent_Eq (lhs: 'ent) (rhs: 'ent)
-| Num_Le "'ent" "'ent"
-| Num_Lt "'ent" "'ent"
-
-
-datatype ('x, atoms: 'a) GD = 
-  Atom 'a
-| Bot
-| Not "('x, 'a) GD"
-| And "('x, 'a) GD" "('x, 'a) GD"
-| Or "('x, 'a) GD" "('x, 'a) GD"
-| Imp "('x, 'a) GD" "('x, 'a) GD"
-| ForAll 'x "('x, 'a) GD"
-| Exists 'x "('x, 'a) GD"
-
-datatype ('x, 'a) pre_GD =
-  PrefGD "pref option" "('x, 'a) GD"
-| ForAll 'x "('x, 'a) pre_GD"
-| And "('x, 'a) pre_GD" "('x, 'a) pre_GD"
-
-
-datatype ('x, atoms: 'a) timed_GD =
-  OverAll "('x, 'a) GD"
-| AtStart "('x, 'a) GD"
-| AtEnd "('x, 'a) GD"
-
-datatype ('x, atoms: 'a) da_GD =
-  ForAll "'x" "('x, 'a) da_GD"
-| And "('x, 'a) da_GD" "('x, 'a) da_GD"
-| PrefTimedGD "pref option" "('x, 'a) timed_GD"
-
-datatype upd_op = 
-  Assign
-| ScaleUp
-| ScaleDown
-| Increase
-| Decrease
-
-datatype (ent: 'ent) of_upd = Fun_Upd upd_op func "'ent list" (ret_val: "'ent option")
-
-datatype 'ent update =
-  S_FU "'ent of_upd"
-| S_Add "'ent atom"
-| S_Del "'ent atom"
-
-datatype ('x, 'ent) effect =
-  Eff "'ent update"
-| Eff_And "('x, 'ent) effect list"
-| Eff_All 'x "('x, 'ent) effect"
-| Eff_When "('x, 'ent atom) GD" "('x, 'ent) effect"
-
-
-datatype 'ent f_exp_t = 
-  Time
-| MultTime "'ent term"
-
-datatype 'ent timed_effect = 
-  DUpd_At_Start "'ent update"
-| DUpd_At_End "'ent update"
-| DurScaleUp func "'ent list" "'ent f_exp_t"
-| DurScaleDown func "'ent list" "'ent f_exp_t"
-
-datatype ('x, 'ent) durative_effect =
-  Timed_Effect "'ent timed_effect"
-| DEff_And "('x, 'ent) durative_effect" "('x, 'ent) durative_effect" 
-| DEff_All 'x "('x, 'ent) durative_effect"
-| DEff_When "('x, 'ent atom) da_GD" "'ent timed_effect"
-  
-datatype ('t) simple_action = Simple_Action
-  (name: name)
-  (parameters: "(variable \<times> type) list")
-  (precondition: "((variable \<times> type) list, 't atom) pre_GD")
-  (effect: "((variable \<times> type) list, 't) effect")
-
-type_synonym ast_pre_GD = "((variable \<times> type) list, variable term atom) pre_GD"
-type_synonym ast_simple_effect = "((variable \<times> type) list, variable term) effect"
-type_synonym ast_simple_action = "variable term simple_action"
-
-datatype 'ent duration_constraint = 
-  DurLe "'ent term"
-| DurGe "'ent term"
-| DurEq "'ent term"
-
-datatype ('t) durative_action = 
-  Durative_Action 
-    (name: name)
-    (duration: "'t duration_constraint list")
-    (parameters: "(variable \<times> type) list")
-    (condition: "((variable \<times> type) list, 't atom) da_GD")
-    (effect: "((variable \<times> type) list, 't) durative_effect")
-
-type_synonym ast_da_GD = "((variable \<times> type) list, variable term atom) da_GD"
-type_synonym ast_durative_effect = "((variable \<times> type) list, variable term) durative_effect"
-type_synonym ast_durative_action = "variable term durative_action"
-
-datatype ast_action = 
-  SA "var_num term simple_action"
-  | DA "var_num_dur term durative_action"
-
-datatype pred_decl = PredDecl
-  (predicate: pred)
-  (argTs: "type list")
-
-datatype obj_fun_decl = ObjFunDecl (of_name: func) "type list" type
-
-datatype derived_pred = 
-  DerivedPred pred 
-    (params: "(variable \<times> type) list")
-    ast_pre_GD
-
-datatype ast_domain = Domain 
-  (types: "(name \<times> name) list") \<comment> \<open> \<open>(type, supertype)\<close> declarations. \<close>
-  ("consts": "(object \<times> type) list")
-  (preds: "pred_decl list")
-  (funs: "obj_fun_decl list")
-  (actions: "ast_action list")
-  (derived: "derived_pred list")
-
-datatype init_asmt = 
-  At rat "object atom"
-  | NotAt rat "object atom"
-  | ObjAsmt func "object list" object
-  | NumAsmt func "object list" rat
-
-
+(* 
 (* This is used for constraints *)
 datatype ('x, atoms: 'a) ltl_form = 
   Atom 'a
@@ -192,6 +39,163 @@ datatype metric_f_exp =
   | Number rat
   | FFun func "object list"
   | IsViolated pref
+ *)
+  
+type_synonym name = String.literal
+
+type_synonym pred = name
+type_synonym func = name
+type_synonym pref = name
+
+datatype type = Either (primitives: "name list") | Number
+datatype variable = Variable (var_name: name)
+datatype object = name: Object (obj_name: name)
+
+(* When we parse, we cannot know whether a simple name is an object or function. Thus,
+  AST types do not have objects*)
+datatype var_num = Var variable | Num rat 
+datatype var_num_dur = Var variable | Num rat | Duration
+
+(* Symbols represent one value, which can be determined independently of the state. 
+    We cannot directly parse these, because objects and functions (in terms) are just strings.
+    Therefore, these only occur after we have checked the function and object type declarations
+    for well-formedness and disambiguated terms. *)
+datatype instant_symbol = Var variable | Const object | Num rat
+datatype symbol = Var variable | Const object | Num rat | Duration
+
+(* When terms are grounded, these are the entities *)
+datatype entity = Const object | Num rat
+
+
+datatype (sym: 'sym) "term" = 
+  Sym 'sym
+| Fun func (arguments: "'sym term list") 
+
+datatype (ent: 'ent) atom = 
+  Pred (pred: pred) (arguments: "'ent list")
+| Ent_Eq (lhs: 'ent) (rhs: 'ent)
+| Num_Le "'ent" "'ent"
+| Num_Lt "'ent" "'ent"
+
+datatype ('x, atoms: 'a) GD = 
+  Atom 'a
+| Bot
+| Not "('x, 'a) GD"
+| And "('x, 'a) GD" "('x, 'a) GD"
+| Or "('x, 'a) GD" "('x, 'a) GD"
+| Imp "('x, 'a) GD" "('x, 'a) GD"
+| ForAll 'x "('x, 'a) GD"
+| Exists 'x "('x, 'a) GD"
+
+datatype ('x, 'a) pre_GD =
+  PrefGD "pref option" "('x, 'a) GD"
+| ForAll 'x "('x, 'a) pre_GD"
+| And "('x, 'a) pre_GD" "('x, 'a) pre_GD"
+
+datatype ('x, atoms: 'a) timed_GD =
+  OverAll "('x, 'a) GD"
+| AtStart "('x, 'a) GD"
+| AtEnd "('x, 'a) GD"
+
+datatype ('x, atoms: 'a) da_GD =
+  ForAll "'x" "('x, 'a) da_GD"
+| And "('x, 'a) da_GD" "('x, 'a) da_GD"
+| PrefTimedGD "pref option" "('x, 'a) timed_GD"
+
+datatype upd_op = 
+  Assign
+| ScaleUp
+| ScaleDown
+| Increase
+| Decrease
+
+datatype (ent: 'ent) f_upd = Fun_Upd upd_op func "'ent list" (ret_val: "'ent option")
+
+datatype 'ent update =
+  S_FU "'ent f_upd"
+| S_Add "'ent atom"
+| S_Del "'ent atom"
+
+datatype ('x, 'ent) effect =
+  Eff "'ent update"
+| Eff_And "('x, 'ent) effect list"
+| Eff_All 'x "('x, 'ent) effect"
+| Eff_When "('x, 'ent atom) GD" "('x, 'ent) effect"
+
+datatype f_exp_t = 
+  Time
+  | MultTime "var_num term"
+
+datatype 'ent timed_effect = 
+  Upd_At_Start "'ent update"
+| Upd_At_End "'ent update"
+| ContScaleUp func "'ent list" f_exp_t
+| ContScaleDown func "'ent list" f_exp_t
+
+datatype ('x, 'ent) durative_effect =
+  Timed_Effect "'ent timed_effect"
+| DEff_And "('x, 'ent) durative_effect" "('x, 'ent) durative_effect" 
+| DEff_All 'x "('x, 'ent) durative_effect"
+| DEff_When "('x, 'ent atom) da_GD" "'ent timed_effect"
+  
+datatype ('t) simple_action = Simple_Action
+  (name: name)
+  (parameters: "(variable \<times> type) list")
+  (precondition: "((variable \<times> type) list, 't atom) pre_GD")
+  (effect: "((variable \<times> type) list, 't) effect option")
+
+type_synonym ast_pre_GD = "((variable \<times> type) list, var_num term atom) pre_GD"
+type_synonym ast_simple_effect = "((variable \<times> type) list, var_num term) effect"
+
+type_synonym ast_simple_action = "var_num term simple_action"
+
+type_synonym ast_simple_duration_constraint = "var_num_dur term atom"
+
+datatype 't timed_atom =
+  AtStart "'t atom"
+  | AtEnd "'t atom"
+
+type_synonym 't duration_constraint = "'t timed_atom"
+
+type_synonym ast_duration_constraint = "var_num_dur duration_constraint"
+type_synonym ast_da_GD = "((variable \<times> type) list, var_num term atom) da_GD"
+type_synonym ast_durative_effect = "((variable \<times> type) list, var_num_dur term) durative_effect"
+
+datatype ast_durative_action = 
+  Durative_Action 
+    (name: name)
+    (duration: "ast_duration_constraint list")
+    (parameters: "(variable \<times> type) list")
+    (condition: "ast_da_GD")
+    (effect: "ast_durative_effect")
+
+
+datatype ast_action = 
+  SA "ast_simple_action"
+  | DA "ast_durative_action"
+
+datatype pred_decl = PredDecl
+  (predicate: pred)
+  (argTs: "type list")
+
+datatype fun_decl = FunDecl (of_name: func) "type list" type
+
+datatype derived_pred = 
+  DerivedPred pred (params: "(variable \<times> type) list") ast_pre_GD
+
+datatype ast_domain = Domain 
+  (types: "(name \<times> name) list") \<comment> \<open> \<open>(type, supertype)\<close> declarations. \<close>
+  ("consts": "(object \<times> type) list")
+  (preds: "pred_decl list")
+  (funs: "fun_decl list")
+  (actions: "ast_action list")
+  (derived: "derived_pred list")
+(*   (constraints: "constraint list") *)
+
+datatype init_asmt = 
+  At rat "object atom"
+  | NotAt rat "object atom"
+  | FunAsmt func "object list" entity
 
 text \<open>A problem consists of a domain, a list of objects,
   a description of the initial state, and a description of the goal state.\<close>
@@ -200,7 +204,7 @@ datatype ast_problem = Problem
   (init_asmts: "init_asmt list")
   (objects: "(object \<times> type) list")
   (goal: "ast_pre_GD")
-  (constraints: "constraint list")
+(*   (constraints: "constraint list") *)
 
 
 subsubsection \<open>Plans\<close>
@@ -208,7 +212,7 @@ type_synonym time = rat
 
 datatype plan_action = 
   Simple_Plan_Action (name: name) (arguments: "object list")
-| Durative_Plan_Action (name: name) (arguments: "object list") (duration: "time option")
+| Durative_Plan_Action (name: name) (arguments: "object list") (duration: "time")
 
 type_synonym plan = "(time \<times> plan_action) list"
 
