PDDL-sema/States.thy
@@ -1,142 +1,68 @@
 theory States
-  imports Terms "Propositional_Proof_Systems.Formulas"
+  imports Terms
 begin
 
 
-type_synonym 'sym num_fun_interpretation = "'sym term f_exp \<rightharpoonup> 'sym term f_exp"
-datatype 'sym state = 
-  State (term_int: "'sym function_interpretation") 
-        (num_term_int: "'sym num_fun_interpretation")
-        (true_preds: "'sym term atom set") 
-        (false_preds: "'sym term atom set")
+
+datatype state = 
+  State (fun_int: "entity function_interpretation") 
+        (true_preds: "entity term atom set") 
+        (false_preds: "entity term atom set")
 
 
-fun nf_f_exp::"'sym function_interpretation 
-  \<Rightarrow> 'sym num_fun_interpretation 
-  \<Rightarrow> 'sym term f_exp \<Rightarrow> bool" where
-"nf_f_exp fi nfi e = (
-  nfi e = None
-\<and> (case e of 
-    (f_exp.NFun f as) \<Rightarrow> list_all (nf_term fi) as
-  | (f_exp.Num _)     \<Rightarrow> True
-  | (f_exp.Neg a)     \<Rightarrow> nf_f_exp fi nfi a
-  | (f_exp.Add a b)   \<Rightarrow> nf_f_exp fi nfi a \<and> nf_f_exp fi nfi b
-  | (f_exp.Sub a b)   \<Rightarrow> nf_f_exp fi nfi a \<and> nf_f_exp fi nfi b
-  | (f_exp.Mult a b)   \<Rightarrow> nf_f_exp fi nfi a \<and> nf_f_exp fi nfi b
-  | (f_exp.Div a b)   \<Rightarrow> nf_f_exp fi nfi a \<and> nf_f_exp fi nfi b
-))"
+definition nf_pred::"'ent function_interpretation \<Rightarrow> 'ent term atom \<Rightarrow> bool" where
+  "nf_pred fi p = (\<forall>t \<in> (atom.ent p). nf_term fi t)"
 
-
-abbreviation n_nfi::"'sym function_interpretation \<Rightarrow>'sym num_fun_interpretation \<Rightarrow> bool" where
-  "n_nfi fi nfi \<equiv> (\<forall>(l, r) \<in> Map.graph nfi. nf_f_exp fi nfi l \<and> nf_f_exp fi nfi r)"
+fun n_state::"state \<Rightarrow> bool" where
+  "n_state (State i t f) = (n_fi i \<and> (\<forall>p \<in> t. nf_pred i p) \<and> (\<forall>p \<in> f. nf_pred i p))"
 
 context
-  fixes fi::"'sym function_interpretation" 
-    and nfi::"'sym num_fun_interpretation"
-    and tp::"'sym term atom set"
-    and fp::"'sym term atom set"
-  assumes n_fi: "n_fi fi"
-      and nf_nfi: "n_nfi fi nfi"
-      and nf_tp: "\<forall>a \<in> tp. \<forall>t \<in> (atom.ent a). nf_term fi t"
-      and nf_fp: "\<forall>a \<in> fp. \<forall>t \<in> (atom.ent a). nf_term fi t"
+  fixes s::state
+  assumes n_state: "n_state s"
 begin
 
-abbreviation "nt \<equiv> normalise_term fi"
-abbreviation "ce \<equiv> check_eq fi"
+abbreviation "nt \<equiv> normalise_term (fun_int s)"
+abbreviation "ce \<equiv> check_eq (fun_int s)"
 
-(* Arithmetic simplifications could be applied here but are not. *)
-fun eval_f_exp::"'sym term f_exp \<Rightarrow> 'sym term f_exp" where
-  "eval_f_exp (f_exp.NFun f as) = (
-      let as' = map nt  as
-      in (case nfi (f_exp.NFun f as') of
-        Some v  \<Rightarrow> v
-      | None    \<Rightarrow> f_exp.NFun f as')
-    )"
-| "eval_f_exp (f_exp.Num n) = f_exp.Num n"
-| "eval_f_exp (f_exp.Neg x) =
-    (case x of
-      f_exp.Num n   \<Rightarrow> f_exp.Num (-n)
-    | x             \<Rightarrow> f_exp.Neg x)"
-| "eval_f_exp (f_exp.Add a b) = 
-    (case (a, b) of
-      (f_exp.Num a', f_exp.Num b')  \<Rightarrow> f_exp.Num (a' + b')
-    | (a, b)                        \<Rightarrow> f_exp.Add a b)"
-| "eval_f_exp (f_exp.Sub a b) = 
-    (case (a, b) of
-      (f_exp.Num a', f_exp.Num b')  \<Rightarrow> f_exp.Num (a' - b')
-    | (a, b)                        \<Rightarrow> f_exp.Sub a b)"
-| "eval_f_exp (f_exp.Mult a b) = 
-    (case (a, b) of
-      (f_exp.Num a', f_exp.Num b')  \<Rightarrow> f_exp.Num (a' * b')
-    | (a, b)                        \<Rightarrow> f_exp.Mult a b)"
-| "eval_f_exp (f_exp.Div a b) = 
-    (case (a, b) of
-      (f_exp.Num a', f_exp.Num b')  \<Rightarrow> if (b' \<noteq> 0) then f_exp.Num (a' / b') else f_exp.Div a b
-    | (a, b)                        \<Rightarrow> f_exp.Div a b)"
+definition check_lt::"entity term \<Rightarrow> entity term \<Rightarrow> bool option" where
+  "check_lt a b \<equiv> (case (nt a, nt b) of
+    (Sym (entity.Num a'), Sym (entity.Num b')) \<Rightarrow> Some (a' \<le> b')
+  | (a', b')                                   \<Rightarrow> if (a' = b') then Some True else None)"
 
-
-(* We could capture more cases of numeric (in-)equalities using rewrite rules, 
-    but they are not trivial *)
-
-(* Derived predicates make PDDL as expressive as an extended logic programming language. *)
-fun atom_sem::"'sym term atom \<Rightarrow> bool option" where
+(* Derived predicates make PDDL as expressive as an extended logic programming language. 
+  Should we implement them? *)
+fun atom_sem::"entity term atom \<Rightarrow> bool option" where
   "atom_sem (Ent_Eq a b) = (if (ce a b) then Some True else None)"
-| "atom_sem (Num_Eq a b) = 
-    (case (eval_f_exp a, eval_f_exp b) of
-      (f_exp.Num a', f_exp.Num b')  \<Rightarrow> Some (a' = b')
-    | (a', b')                      \<Rightarrow> if (a' = b') then Some True else None)"
-| "atom_sem (Num_Le a b) = 
-    (case (eval_f_exp a, eval_f_exp b) of
-      (f_exp.Num a', f_exp.Num b')  \<Rightarrow> Some (a' \<le> b')
-    | (a', b')                      \<Rightarrow> if (a' = b') then Some True else None)"
-| "atom_sem (Num_Lt a b) = 
-    (case (eval_f_exp a, eval_f_exp b) of
-      (f_exp.Num a', f_exp.Num b')  \<Rightarrow> Some (a' < b')
-    | (a', b')                      \<Rightarrow> if (a' = b') then Some False else None)"
+| "atom_sem (Num_Le a b) = check_lt a b"
+| "atom_sem (Num_Lt a b) = map_option (\<lambda>x. \<not>x) (check_lt b a)"
 | "atom_sem (Pred p as) = 
     (let as' = map nt as in
-      if      (Pred p as') \<in> tp then Some True 
-      else if (Pred p as') \<in> fp then Some False 
+      if      (Pred p as') \<in> (true_preds s) then Some True 
+      else if (Pred p as') \<in> (false_preds s) then Some False 
       else None)"
 end
 
 context 
-  fixes fi::"object function_interpretation"
-    and nfi::"object num_fun_interpretation"
-    and tp::"object term atom set"
-    and fp::"object term atom set"
+  fixes s::state
     and ty_dom::"type \<Rightarrow> object list"
-  assumes n_fi: "n_fi fi"
-      and nf_nfi: "n_nfi fi nfi"
-      and nf_tp: "\<forall>a \<in> tp. \<forall>t \<in> (atom.ent a). nf_term fi t"
-      and nf_fp: "\<forall>a \<in> fp. \<forall>t \<in> (atom.ent a). nf_term fi t"
+  assumes n_state: "n_state s"
 begin
 
-abbreviation "at_sem \<equiv> atom_sem fi nfi tp fp"
+abbreviation "at_sem \<equiv> atom_sem s"
 text \<open>The variables in a symbol\<close>
-fun sym_vars where
-  "sym_vars (Var x) = {x}" 
-| "sym_vars (Const c) = {}"
+fun sym_vars::"symbol \<Rightarrow> variable set" where
+  "sym_vars (symbol.Var x) = {x}" 
+| "sym_vars _ = {}"
 
 fun term_vars::"symbol term \<Rightarrow> variable set" where
   "term_vars (Sym x) = sym_vars x"
 | "term_vars (Fun f as) = fold (\<union>) (map term_vars as) {}"
 
-fun f_exp_vars::"symbol term f_exp \<Rightarrow> variable set" where
-  "f_exp_vars (f_exp.NFun f as) = fold (\<union>) (map term_vars as) {}"
-| "f_exp_vars (f_exp.Num n) = {}"
-| "f_exp_vars (f_exp.Neg e) = f_exp_vars e"
-| "f_exp_vars (f_exp.Add a b) = f_exp_vars a \<union> f_exp_vars b"
-| "f_exp_vars (f_exp.Sub a b) = f_exp_vars a \<union> f_exp_vars b"
-| "f_exp_vars (f_exp.Mult a b) = f_exp_vars a \<union> f_exp_vars b"
-| "f_exp_vars (f_exp.Div a b) = f_exp_vars a \<union> f_exp_vars b"
-
 fun atom_vars::"symbol term atom \<Rightarrow> variable set" where
   "atom_vars (Pred p as) = fold (\<union>) (map term_vars as) {}"
 | "atom_vars (Ent_Eq a b) = term_vars a \<union> term_vars b"
-| "atom_vars (Num_Eq a b) = f_exp_vars a \<union> f_exp_vars b"
-| "atom_vars (Num_Le a b) = f_exp_vars a \<union> f_exp_vars b"
-| "atom_vars (Num_Lt a b) = f_exp_vars a \<union> f_exp_vars b"
+| "atom_vars (Num_Le a b) = term_vars a \<union> term_vars b"
+| "atom_vars (Num_Lt a b) = term_vars a \<union> term_vars b"
 
 fun f_vars::"((variable \<times> 'x) list, symbol term atom) GD \<Rightarrow> variable set" where
   "f_vars (GD.Atom a) = atom_vars a"
@@ -158,7 +84,7 @@ fun f_vars'::"(variable \<times> 'x, symbol term atom) GD \<Rightarrow> variable
 | "f_vars' (GD.ForAll (v, os) f) = f_vars' f - {v}"
 | "f_vars' (GD.Exists (v, os) f) = f_vars' f - {v}"
 
-fun ground_GD_sem::"(unit, object term atom) GD \<Rightarrow> bool option" where
+fun ground_GD_sem::"(unit, entity term atom) GD \<Rightarrow> bool option" where
   "ground_GD_sem (GD.Atom a)   = at_sem a"
 | "ground_GD_sem GD.Bot        = Some False"
 | "ground_GD_sem (GD.Not gd)   = map_option (\<lambda>x. \<not>x) (ground_GD_sem gd)"
@@ -185,19 +111,21 @@ fun BigOr::"('a, 'b) GD list \<Rightarrow> ('a, 'b) GD" where
   "BigOr [] = GD.Bot"
 | "BigOr (f#fs) = GD.Or f (BigOr fs)"
 
-fun subst_sym_with_obj where
-  "subst_sym_with_obj psubst (Var x) = psubst x"
-| "subst_sym_with_obj psubst (Const c) = c"
+fun inst_sym::"(variable \<Rightarrow> object) \<Rightarrow> time \<Rightarrow> symbol \<Rightarrow> entity" where
+  "inst_sym f dur (symbol.Var x) = entity.Const (f x)"
+| "inst_sym f dur (symbol.Const c) = entity.Const c"
+| "inst_sym f dur (symbol.Num n) = entity.Num n"
+| "inst_sym f dur (symbol.Duration) = entity.Num dur"
 
-fun ground_GD::"(symbol \<Rightarrow> object) \<Rightarrow> (variable \<times> (object list), symbol term atom) GD \<Rightarrow> (unit, object term atom) GD" where
+fun ground_GD::"(symbol \<Rightarrow> entity) \<Rightarrow> (variable \<times> (object list), symbol term atom) GD \<Rightarrow> (unit, entity term atom) GD" where
   "ground_GD f (GD.Atom a) = GD.Atom (map_atom (map_term f) a)"
 | "ground_GD f GD.Bot = GD.Bot"
 | "ground_GD f (GD.Not x) = GD.Not (ground_GD f x)"
 | "ground_GD f (GD.And x y) = GD.And (ground_GD f x) (ground_GD f y)"
 | "ground_GD f (GD.Or x y) = GD.Or (ground_GD f x) (ground_GD f y)"
 | "ground_GD f (GD.Imp x y) = GD.Imp (ground_GD f x) (ground_GD f y)"
-| "ground_GD f (GD.ForAll (v, os) x) = (if (v \<notin> f_vars' x \<and> os \<noteq> []) then ground_GD f x else BigAnd (map (\<lambda>obj. ground_GD (f((Var v):=obj)) x) os))"
-| "ground_GD f (GD.Exists (v, os) x) = (if (v \<notin> f_vars' x \<and> os \<noteq> []) then ground_GD f x else BigOr (map (\<lambda>obj. ground_GD (f((Var v):=obj)) x) os))"
+| "ground_GD f (GD.ForAll (v, os) x) = (if (v \<notin> f_vars' x \<and> os \<noteq> []) then ground_GD f x else BigAnd (map (\<lambda>obj. ground_GD (f((symbol.Var v):=(entity.Const obj))) x) os))"
+| "ground_GD f (GD.Exists (v, os) x) = (if (v \<notin> f_vars' x \<and> os \<noteq> []) then ground_GD f x else BigOr (map (\<lambda>obj. ground_GD (f((symbol.Var v):=(entity.Const obj))) x) os))"
 
 abbreviation replace_types_with_objects where
   "replace_types_with_objects \<equiv> map_GD (\<lambda>(v, t). (v, ty_dom t)) id"
@@ -214,7 +142,7 @@ fun split_quant::"(('a \<times> 'b) list, 'c) GD \<Rightarrow> ('a \<times> 'b, 
 
 text \<open>This is the process of instantiating and executing an action.\<close>
 
-definition GD_sem::"(symbol \<Rightarrow> object) \<Rightarrow> ((variable \<times> type) list, symbol term atom) GD \<Rightarrow> bool option" where
+definition GD_sem::"(symbol \<Rightarrow> entity) \<Rightarrow> ((variable \<times> type) list, symbol term atom) GD \<Rightarrow> bool option" where
   "GD_sem f \<phi> = ground_GD_sem (ground_GD f (replace_types_with_objects (split_quant \<phi>)))"
 
 end
